\subsection{Zadanie 9}

$$
\int\limits_{-\infty}^{\infty}(x-m)^{2}g(x)dx= \int\limits_{-\infty}^{\infty}x^{2}g(x)dx-m^{2}
$$

\begin{enumerate}[label=(\alph*)]
\item
$$ [0,1] $$
$$ E(x)=\frac{1}{2} $$
$$
\int\limits_{0}^{1}x^{2}dx - \frac{1}{4} =
\left. \frac{1}{3}x^{3} \right|_{0}^{1} - \frac{1}{4} = \frac{1}{12}
$$

\item
$$[a,b]E(x)=\frac{(a+b)}{2}$$

$$
\int\limits_{a}^{b}x^{2}\frac{1}{b-a}dx - \frac{(a+b)^{2}}{4} =
\left. \frac{1}{b-a} * \frac{1}{3}x^{3} \right|_{a}^{b} - \frac{(a+b)}{4} =
\frac{1}{3} * \frac{1}{b-a} * (b-a)^{3} - \frac{(a+b)^{2}}{4}=
$$

$$
= \frac{1}{3} * \frac{(b-a)(b^{2} + ab + a^{2})}{b - a} - \frac{a^{2}+ 2ab +
b^{2}}{4} =
$$
$$
\frac{4(b^{2} + ab + a^{2})}{12} - \frac{3(b^{2} + 2ab + a^{2})}{12} =
\frac{b^{2} - 2ab + a^{2}}{12}= \frac{(b - a)^{2}}{12}
$$
\end{enumerate}
